DY/ALaCarte/DecidableEq.lean
@@ -13,8 +13,8 @@ theorem BareContainer.decideEquality.aux
   (h1: ∀ x, x ∈ l1 → sizeOf x < max (sizeOf l1) (sizeOf l2))
   (h2: ∀ x, x ∈ l2 → sizeOf x < max (sizeOf l1) (sizeOf l2))
   : (l1.attachWith _ h1 = l2.attachWith _ h2) = (l1 = l2)
-  := by
-    grind [Array.unattach_attachWith]
+:= by
+  grind [Array.unattach_attachWith]
 
 def BareContainer.decideEquality
   {CtorId} {ctors: Ctors CtorId}
@@ -22,31 +22,31 @@ def BareContainer.decideEquality
   [∀ id, DecidableEq (ctors id).Data]
   (x1 x2: BareContainer ctors)
   : Decidable (x1 = x2)
-  := by
-    let { id := id1, data := data1, as := as1 } := x1
-    let { id := id2, data := data2, as := as2 } := x2
-    simp only [BareContainer.mk.injEq]
-    by_cases (decide (id1 = id2)) <;> rename_i h_id
-    · simp only [decide_eq_true_eq] at h_id
-      subst h_id
-      simp only [heq_eq_eq, true_and]
-      by_cases (decide (data1 = data2)) <;> rename_i h_data
-      · simp only [decide_eq_true_eq] at h_data
-        subst h_data
-        simp only [true_and]
-        rewrite [← BareContainer.decideEquality.aux]
-        · refine @Array.instDecidableEq _ ?_ _ _
-          intro ⟨x1, h_x1⟩ ⟨x2, h_x2⟩
-          simp only [Subtype.mk.injEq]
-          apply BareContainer.decideEquality
-        all_goals
-        intro x h_x
-        have := Array.sizeOf_lt_of_mem h_x
-        grind
-      · left
-        simp_all
+:= by
+  let { id := id1, data := data1, as := as1 } := x1
+  let { id := id2, data := data2, as := as2 } := x2
+  simp only [BareContainer.mk.injEq]
+  by_cases (decide (id1 = id2)) <;> rename_i h_id
+  · simp only [decide_eq_true_eq] at h_id
+    subst h_id
+    simp only [heq_eq_eq, true_and]
+    by_cases (decide (data1 = data2)) <;> rename_i h_data
+    · simp only [decide_eq_true_eq] at h_data
+      subst h_data
+      simp only [true_and]
+      rewrite [← BareContainer.decideEquality.aux]
+      · refine @Array.instDecidableEq _ ?_ _ _
+        intro ⟨x1, h_x1⟩ ⟨x2, h_x2⟩
+        simp only [Subtype.mk.injEq]
+        apply BareContainer.decideEquality
+      all_goals
+      intro x h_x
+      have := Array.sizeOf_lt_of_mem h_x
+      grind
     · left
       simp_all
+  · left
+    simp_all
 termination_by max (sizeOf x1) (sizeOf x2)
 
 def Container.decideEquality
@@ -55,19 +55,17 @@ def Container.decideEquality
   [∀ id, DecidableEq (ctors id).Data]
   (x1 x2: Container ctors)
   : Decidable (x1 = x2)
-  := by
-    cases x1
-    cases x2
-    rewrite [Subtype.mk.injEq]
-    apply BareContainer.decideEquality
+:= by
+  cases x1
+  cases x2
+  rewrite [Subtype.mk.injEq]
+  apply BareContainer.decideEquality
 
 class RepresentableDecidableEq (f: Type → Type) [FunctorSizeOf f] [Representable f] where
-  ctorid_deq: DecidableEq (Representable.CtorId f)
-  := by
+  ctorid_deq: DecidableEq (Representable.CtorId f) := by
     simp only [DY.ALaCarte.Representable.CtorId]
     exact inferInstance
-  ctor_data_deq: ∀ id, DecidableEq (Representable.ctors (f := f) id).Data
-  := by
+  ctor_data_deq: ∀ id, DecidableEq (Representable.ctors (f := f) id).Data := by
     intro id
     simp only [DY.ALaCarte.Representable.ctors]
     cases id <;>
