DY/ALaCarte/Ordering.lean
@@ -15,8 +15,9 @@ namespace DY.ALaCarte
 
 def Array.attachWithSize
   {α: Type} [SizeOf α]
-  (arr: Array α) (n: Nat) (H : sizeOf arr ≤ n := by grind) : Array {x: α // sizeOf x < n}
-  :=
+  (arr: Array α) (n: Nat) (H : sizeOf arr ≤ n := by grind)
+  : Array {x: α // sizeOf x < n}
+:=
   arr.attachWith (fun x => sizeOf x < n) (by
     intro h h_x
     have := Array.sizeOf_lt_of_mem h_x
@@ -25,8 +26,9 @@ def Array.attachWithSize
 
 def List.attachWithSize
   {α: Type} [SizeOf α]
-  (l: List α) (n: Nat) (H : sizeOf l ≤ n := by grind) : List {x: α // sizeOf x < n}
-  :=
+  (l: List α) (n: Nat) (H : sizeOf l ≤ n := by grind)
+  : List {x: α // sizeOf x < n}
+:=
   l.attachWith (fun x => sizeOf x < n) (by
     intro h h_x
     have := List.sizeOf_lt_of_mem h_x
@@ -37,7 +39,8 @@ theorem Array.attachWithSize_eq_attachWithSize_toList
   {α: Type} [SizeOf α]
   (arr: Array α) (n: Nat) (H : sizeOf arr ≤ n)
   : (Array.attachWithSize arr n H).toList = List.attachWithSize arr.toList n (by cases arr; simp_all; grind)
-  := by rfl
+:= by
+  rfl
 
 
 @[wf_preprocess]
@@ -45,44 +48,45 @@ theorem Array.compareLex_wfParam
   {α: Type} [SizeOf α]
   (cmp: α → α → Ordering) (arr1: Array α) (arr2: Array α)
   : Array.compareLex cmp (wfParam arr1) (wfParam arr2) = Array.compareLex cmp ((Array.attachWithSize arr1 (max (sizeOf arr1) (sizeOf arr2))).unattach) ((Array.attachWithSize arr2 (max (sizeOf arr1) (sizeOf arr2))).unattach)
-  := by
-    cases arr1; rename_i l1
-    cases arr2; rename_i l2
-    simp only [Array.compareLex_eq_compareLex_toList, Array.toList_unattach, Array.attachWithSize_eq_attachWithSize_toList, wfParam, Array.mk.sizeOf_spec]
-    fun_induction List.compareLex cmp l1 l2
-    all_goals
-    conv => rhs; unfold List.compareLex
-    simp_all [List.attachWithSize]
+:= by
+  cases arr1; rename_i l1
+  cases arr2; rename_i l2
+  simp only [Array.compareLex_eq_compareLex_toList, Array.toList_unattach, Array.attachWithSize_eq_attachWithSize_toList, wfParam, Array.mk.sizeOf_spec]
+  fun_induction List.compareLex cmp l1 l2
+  all_goals
+  conv => rhs; unfold List.compareLex
+  simp_all [List.attachWithSize]
 
 theorem List.unattach_eq_nil
   {α: Type u} {P: α → Prop}
   (l: List (Subtype P))
   : l.unattach = [] ↔ l = []
-  := by
-    cases l <;> simp
+:= by
+  cases l <;> simp
 
 @[wf_preprocess]
-theorem Array.compareLex_unattach {P: α → Prop} (cmp: α → α → Ordering)
-    (arr1 arr2 : Array (Subtype P))
-    :
-    Array.compareLex cmp arr1.unattach arr2.unattach =
+theorem Array.compareLex_unattach
+  {P: α → Prop}
+  (cmp: α → α → Ordering)
+  (arr1 arr2 : Array (Subtype P))
+  : Array.compareLex cmp arr1.unattach arr2.unattach =
     Array.compareLex (fun x1 x2 => cmp (wfParam x1.val) (wfParam x2.val)) arr1 arr2
-  := by
-    cases arr1; rename_i l1
-    cases arr2; rename_i l2
-    simp only [List.unattach_toArray, Array.compareLex_eq_compareLex_toList, wfParam]
-    fun_induction List.compareLex (fun x1 x2 => cmp x1.val x2.val) l1 l2
-    · simp [List.compareLex]
-    · unfold List.compareLex
-      split <;> simp_all [List.unattach_eq_nil]
-    · unfold List.compareLex
-      split <;> simp_all [List.unattach_eq_nil]
-    · unfold List.compareLex
-      split <;> simp_all
-    · simp [List.compareLex]
-      split <;> simp_all
-    · unfold List.compareLex
-      split <;> simp_all
+:= by
+  cases arr1; rename_i l1
+  cases arr2; rename_i l2
+  simp only [List.unattach_toArray, Array.compareLex_eq_compareLex_toList, wfParam]
+  fun_induction List.compareLex (fun x1 x2 => cmp x1.val x2.val) l1 l2
+  · simp [List.compareLex]
+  · unfold List.compareLex
+    split <;> simp_all [List.unattach_eq_nil]
+  · unfold List.compareLex
+    split <;> simp_all [List.unattach_eq_nil]
+  · unfold List.compareLex
+    split <;> simp_all
+  · simp [List.compareLex]
+    split <;> simp_all
+  · unfold List.compareLex
+    split <;> simp_all
 
 
 /-
@@ -94,18 +98,18 @@ def BareContainer.compare
   [∀ id, Ord (ctors id).Data]
   (x1 x2: BareContainer ctors)
   : Ordering
-  :=
-    let {id := id1, data := data1, as := as1} := x1
-    let {id := id2, data := data2, as := as2} := x2
-    match h: Ord.compare id1 id2 with
-    | .lt => .lt
-    | .gt => .gt
-    | .eq => by
-      simp at h
-      subst h
-      exact (
-        Ordering.then (Ord.compare data1 data2) (Array.compareLex BareContainer.compare as1 as2)
-      )
+:=
+  let {id := id1, data := data1, as := as1} := x1
+  let {id := id2, data := data2, as := as2} := x2
+  match h: Ord.compare id1 id2 with
+  | .lt => .lt
+  | .gt => .gt
+  | .eq => by
+    simp at h
+    subst h
+    exact (
+      Ordering.then (Ord.compare data1 data2) (Array.compareLex BareContainer.compare as1 as2)
+    )
 termination_by max (sizeOf (self := BareContainer._sizeOf_inst ctors) x1) (sizeOf (self := BareContainer._sizeOf_inst ctors) x2)
 decreasing_by
   simp_all
@@ -118,24 +122,26 @@ theorem List.compareLex.into_attachWithSize.aux
   (h_n: max (sizeOf l1) (sizeOf l2) ≤ n)
   (cmp: α → α → Ordering)
   : List.compareLex cmp l1 l2 = List.compareLex (fun x y => cmp x.val y.val) (List.attachWithSize l1 n) (List.attachWithSize l2 n)
-  := by
-    unfold List.attachWithSize
-    fun_induction List.compareLex
-    <;> simp_all [List.compareLex]
-    simp at h_n --?
-    grind
+:= by
+  unfold List.attachWithSize
+  fun_induction List.compareLex
+  <;> simp_all [List.compareLex]
+  simp at h_n --?
+  grind
 
 def List.compareLex.into_attachWith
   {α: Type} [SizeOf α]
   (l1 l2: List α)
   (cmp: α → α → Ordering)
-  := List.compareLex.into_attachWithSize.aux l1 l2 (max (sizeOf l1) (sizeOf l2)) (by grind) cmp
+:=
+  List.compareLex.into_attachWithSize.aux l1 l2 (max (sizeOf l1) (sizeOf l2)) (by grind) cmp
 
 def List.compareLex.into_attachWith_flip
   {α: Type} [SizeOf α]
   (l1 l2: List α)
   (cmp: α → α → Ordering)
-  := List.compareLex.into_attachWithSize.aux l1 l2 (max (sizeOf l2) (sizeOf l1)) (by grind) cmp
+:=
+  List.compareLex.into_attachWithSize.aux l1 l2 (max (sizeOf l2) (sizeOf l1)) (by grind) cmp
 
 /-
   Theorems about List.compareLex, but without going through the typeclass instances.
@@ -147,10 +153,10 @@ theorem List.compareLex.compare_self
   (h_cmp: ∀ x, cmp x x = .eq)
   (l: List α)
   : List.compareLex cmp l l = .eq
-  := by
-    refine Std.ReflCmp.compare_self (self := @List.instReflCmpCompareLex _ _ ?_)
-    constructor
-    grind
+:= by
+  refine Std.ReflCmp.compare_self (self := @List.instReflCmpCompareLex _ _ ?_)
+  constructor
+  grind
 
 theorem List.compareLex.eq_of_compare
   {α: Type}
@@ -159,12 +165,12 @@ theorem List.compareLex.eq_of_compare
   (h_cmp2: ∀ x1 x2, cmp x1 x2 = .eq → x1 = x2)
   (l1 l2: List α)
   : List.compareLex cmp l1 l2 = .eq → l1 = l2
-  := by
-    refine Std.LawfulEqCmp.eq_of_compare (self := @List.instLawfulEqCmpCompareLex _ _ ?_)
-    refine @Std.LawfulEqCmp.mk _ _ ?_ ?_
-    · constructor
-      grind
+:= by
+  refine Std.LawfulEqCmp.eq_of_compare (self := @List.instLawfulEqCmpCompareLex _ _ ?_)
+  refine @Std.LawfulEqCmp.mk _ _ ?_ ?_
+  · constructor
     grind
+  grind
 
 theorem List.compareLex.eq_swap
   {α: Type}
@@ -172,10 +178,10 @@ theorem List.compareLex.eq_swap
   (h_cmp: ∀ x1 x2, cmp x1 x2 = (cmp x2 x1).swap)
   (l1 l2: List α)
   : List.compareLex cmp l1 l2 = (List.compareLex cmp l2 l1).swap
-  := by
-    refine Std.OrientedCmp.eq_swap (self := @List.instOrientedCmpCompareLex _ _ ?_)
-    constructor
-    grind
+:= by
+  refine Std.OrientedCmp.eq_swap (self := @List.instOrientedCmpCompareLex _ _ ?_)
+  constructor
+  grind
 
 theorem List.compareLex.isLE_trans
   {α: Type}
@@ -184,12 +190,12 @@ theorem List.compareLex.isLE_trans
   (h_cmp2: ∀ x1 x2 x3, (cmp x1 x2).isLE → (cmp x2 x3).isLE → (cmp x1 x3).isLE)
   (l1 l2 l3: List α)
   : (List.compareLex cmp l1 l2).isLE → (List.compareLex cmp l2 l3).isLE → (List.compareLex cmp l1 l3).isLE
-  := by
-    refine Std.TransCmp.isLE_trans (self := @List.instTransCmpCompareLex _ _ ?_)
-    refine @Std.TransCmp.mk _ _ ?_ ?_
-    · constructor
-      grind
+:= by
+  refine Std.TransCmp.isLE_trans (self := @List.instTransCmpCompareLex _ _ ?_)
+  refine @Std.TransCmp.mk _ _ ?_ ?_
+  · constructor
     grind
+  grind
 
 /-
   Theorems on BareContainer.compare
@@ -202,18 +208,18 @@ theorem BareContainer.compare.compare_self
   [∀ id, Std.ReflOrd (ctors id).Data]
   (x: BareContainer ctors)
   : compare x x = .eq
-  := by
-    let {id, data, as} := x
-    unfold BareContainer.compare
-    simp only
-    have id_refl: Ord.compare id id = .eq := by simp
-    rewrite [id_refl]
-    dsimp only
-    simp only [Std.compare_self, Ordering.eq_then]
-    rewrite [Array.compareLex_eq_compareLex_toList, List.compareLex.into_attachWith]
-    apply List.compareLex.compare_self
-    intro
-    apply BareContainer.compare.compare_self
+:= by
+  let {id, data, as} := x
+  unfold BareContainer.compare
+  simp only
+  have id_refl: Ord.compare id id = .eq := by simp
+  rewrite [id_refl]
+  dsimp only
+  simp only [Std.compare_self, Ordering.eq_then]
+  rewrite [Array.compareLex_eq_compareLex_toList, List.compareLex.into_attachWith]
+  apply List.compareLex.compare_self
+  intro
+  apply BareContainer.compare.compare_self
 decreasing_by
   rename_i x
   cases as
@@ -227,8 +233,8 @@ theorem BareContainer.compare.lawful_eq.attachWith_eq
   (h1: ∀ x, x ∈ l1 → sizeOf x < max (sizeOf l1) (sizeOf l2))
   (h2: ∀ x, x ∈ l2 → sizeOf x < max (sizeOf l1) (sizeOf l2))
   : (l1.attachWith _ h1 = l2.attachWith _ h2) = (l1 = l2)
-  := by
-    grind [List.unattach_attachWith]
+:= by
+  grind [List.unattach_attachWith]
 
 theorem BareContainer.compare.eq_of_compare
   {CtorId} {ctors: Ctors CtorId}
@@ -237,35 +243,35 @@ theorem BareContainer.compare.eq_of_compare
   [∀ id, Std.LawfulEqOrd (ctors id).Data]
   (x1 x2: BareContainer ctors)
   : compare x1 x2 = .eq → x1 = x2
-  := by
-    let {id := id1, data := data1, as := { toList := l1 }} := x1
-    let {id := id2, data := data2, as := { toList := l2 }} := x2
-    simp only [BareContainer.compare, BareContainer.mk.injEq]
-    split
-    · simp
-    · simp
-    rename_i heq
-    have heq := Std.LawfulEqOrd.eq_of_compare heq
-    subst heq
-    dsimp only [Ordering.then]
-    split
-    · rename_i heq
-      have := Std.LawfulEqOrd.eq_of_compare heq
-      simp_all only [Std.compare_self, heq_eq_eq, true_and]
-      rewrite [Array.compareLex_eq_compareLex_toList, List.compareLex.into_attachWith]
-      simp only [Array.mk.injEq]
-      rewrite [←BareContainer.compare.lawful_eq.attachWith_eq l1 l2]
-      apply List.compareLex.eq_of_compare
-      · intro
-        apply BareContainer.compare.compare_self
-      · intro ⟨a, h_a⟩ ⟨b, h_b⟩
-        simp only [Subtype.mk.injEq]
-        apply BareContainer.compare.eq_of_compare
-      all_goals
-      intro x h_x
-      have := List.sizeOf_lt_of_mem h_x
-      grind [List.sizeOf_lt_of_mem]
-    · grind
+:= by
+  let {id := id1, data := data1, as := { toList := l1 }} := x1
+  let {id := id2, data := data2, as := { toList := l2 }} := x2
+  simp only [BareContainer.compare, BareContainer.mk.injEq]
+  split
+  · simp
+  · simp
+  rename_i heq
+  have heq := Std.LawfulEqOrd.eq_of_compare heq
+  subst heq
+  dsimp only [Ordering.then]
+  split
+  · rename_i heq
+    have := Std.LawfulEqOrd.eq_of_compare heq
+    simp_all only [Std.compare_self, heq_eq_eq, true_and]
+    rewrite [Array.compareLex_eq_compareLex_toList, List.compareLex.into_attachWith]
+    simp only [Array.mk.injEq]
+    rewrite [←BareContainer.compare.lawful_eq.attachWith_eq l1 l2]
+    apply List.compareLex.eq_of_compare
+    · intro
+      apply BareContainer.compare.compare_self
+    · intro ⟨a, h_a⟩ ⟨b, h_b⟩
+      simp only [Subtype.mk.injEq]
+      apply BareContainer.compare.eq_of_compare
+    all_goals
+    intro x h_x
+    have := List.sizeOf_lt_of_mem h_x
+    grind [List.sizeOf_lt_of_mem]
+  · grind
 termination_by max (sizeOf x1) (sizeOf x2)
 decreasing_by
   simp
@@ -279,36 +285,36 @@ theorem BareContainer.compare.eq_swap
   [∀ id, Std.OrientedOrd (ctors id).Data]
   (x1 x2: BareContainer ctors)
   : compare x1 x2 = (compare x2 x1).swap
-  := by
-    let {id := id1, data := data1, as := { toList := l1 }} := x1
-    let {id := id2, data := data2, as := { toList := l2 }} := x2
-    simp only [BareContainer.compare]
-    have id_swap: Ord.compare id1 id2 = (Ord.compare id2 id1).swap := Std.OrientedOrd.eq_swap
+:= by
+  let {id := id1, data := data1, as := { toList := l1 }} := x1
+  let {id := id2, data := data2, as := { toList := l2 }} := x2
+  simp only [BareContainer.compare]
+  have id_swap: Ord.compare id1 id2 = (Ord.compare id2 id1).swap := Std.OrientedOrd.eq_swap
+  split
+  · grind
+  · grind
+  rename_i heq
+  have heq := Std.LawfulEqOrd.eq_of_compare heq
+  subst heq
+  dsimp only [Ordering.then]
+  have data_swap: Ord.compare data1 data2 = (Ord.compare data2 data1).swap := Std.OrientedOrd.eq_swap
+  split
+  · simp only [Array.compareLex_eq_compareLex_toList]
+    rewrite (occs := [2]) [List.compareLex.into_attachWith_flip]
+    rewrite (occs := [1]) [List.compareLex.into_attachWith]
+    have := List.compareLex.eq_swap (fun x y => x.val.compare y.val) (by
+      intro ⟨a, h_a⟩ ⟨b, h_b⟩
+      dsimp only
+      apply BareContainer.compare.eq_swap
+    ) (List.attachWithSize l1 (max (sizeOf l1) (sizeOf l2))) (List.attachWithSize l2 (max (sizeOf l1) (sizeOf l2)))
     split
     · grind
     · grind
-    rename_i heq
-    have heq := Std.LawfulEqOrd.eq_of_compare heq
-    subst heq
-    dsimp only [Ordering.then]
-    have data_swap: Ord.compare data1 data2 = (Ord.compare data2 data1).swap := Std.OrientedOrd.eq_swap
     split
-    · simp only [Array.compareLex_eq_compareLex_toList]
-      rewrite (occs := [2]) [List.compareLex.into_attachWith_flip]
-      rewrite (occs := [1]) [List.compareLex.into_attachWith]
-      have := List.compareLex.eq_swap (fun x y => x.val.compare y.val) (by
-        intro ⟨a, h_a⟩ ⟨b, h_b⟩
-        dsimp only
-        apply BareContainer.compare.eq_swap
-      ) (List.attachWithSize l1 (max (sizeOf l1) (sizeOf l2))) (List.attachWithSize l2 (max (sizeOf l1) (sizeOf l2)))
-      split
-      · grind
-      · grind
-      split
-      · grind
-      · simp [Ordering.swap] at data_swap
-        grind
     · grind
+    · simp [Ordering.swap] at data_swap
+      grind
+  · grind
 termination_by max (sizeOf x1) (sizeOf x2)
 decreasing_by
   simp
@@ -321,9 +327,9 @@ theorem transLtToLe
   (x y z: a)
   (h_translt: (r x y) = .lt → (r y z) = .lt → (r x z) = .lt)
   : (r x y).isLE → (r y z).isLE → (r x z).isLE
-  := by
-    simp only [Ordering.isLE]
-    grind [cases Ordering]
+:= by
+  simp only [Ordering.isLE]
+  grind [cases Ordering]
 
 theorem transLeToLt
   {a: Type u}
@@ -333,10 +339,10 @@ theorem transLeToLt
   (x y z: a)
   (h_transle: (r x y).isLE → (r y z).isLE → (r x z).isLE)
   : (r x y) = .lt → (r y z) = .lt → (r x z) = .lt
-  := by
-    unfold Ordering.swap at h_swap
-    unfold Ordering.isLE at h_transle
-    grind [cases Ordering]
+:= by
+  unfold Ordering.swap at h_swap
+  unfold Ordering.isLE at h_transle
+  grind [cases Ordering]
 
 theorem BareContainer.compare.isLE_trans
   {CtorId} {ctors: Ctors CtorId}
@@ -347,61 +353,61 @@ theorem BareContainer.compare.isLE_trans
   [∀ id, Std.TransOrd (ctors id).Data]
   (x1 x2 x3: BareContainer ctors)
   : (compare x1 x2).isLE → (compare x2 x3).isLE → (compare x1 x3).isLE
-  := by
-    apply transLtToLe
-    · apply BareContainer.compare.eq_of_compare
-    let {id := id1, data := data1, as := { toList := l1} } := x1
-    let {id := id2, data := data2, as := { toList := l2} } := x2
-    let {id := id3, data := data3, as := { toList := l3} } := x3
-    simp only [BareContainer.compare, Ordering.then]
-    intro h12 h23
-    split at h12 <;> rename_i h_id12
-    · split at h23 <;> rename_i h_id23
-      · have := Std.TransCmp.lt_trans h_id12 h_id23
-        grind
-      · contradiction
-      · grind
+:= by
+  apply transLtToLe
+  · apply BareContainer.compare.eq_of_compare
+  let {id := id1, data := data1, as := { toList := l1} } := x1
+  let {id := id2, data := data2, as := { toList := l2} } := x2
+  let {id := id3, data := data3, as := { toList := l3} } := x3
+  simp only [BareContainer.compare, Ordering.then]
+  intro h12 h23
+  split at h12 <;> rename_i h_id12
+  · split at h23 <;> rename_i h_id23
+    · have := Std.TransCmp.lt_trans h_id12 h_id23
+      grind
     · contradiction
-    split at h23 <;> rename_i h_id23
     · grind
-    · contradiction
-    have h_id12_eq := Std.LawfulEqOrd.eq_of_compare h_id12
-    have h_id23_eq := Std.LawfulEqOrd.eq_of_compare h_id23
-    subst h_id12_eq
-    subst h_id23_eq
-    dsimp only at *
-    rewrite [h_id12]
-    dsimp only
-    split at h12 <;> rename_i h_data12
-    · split at h23 <;> rename_i h_data23
-      · have h_data12_eq := Std.LawfulEqOrd.eq_of_compare h_data12
-        have h_data23_eq := Std.LawfulEqOrd.eq_of_compare h_data23
-        subst h_data12_eq
-        subst h_data23_eq
-        simp only [h_data12]
-        revert h12 h23
-        simp only [Array.compareLex_eq_compareLex_toList]
-        apply transLeToLt
-        · apply List.compareLex.eq_of_compare
-          · apply BareContainer.compare.compare_self
-          · apply BareContainer.compare.eq_of_compare
-        · apply List.compareLex.eq_swap
-          apply BareContainer.compare.eq_swap
-        simp only [List.compareLex.into_attachWithSize.aux l1 l2 (max (max (sizeOf l1) (sizeOf l2)) (sizeOf l3)) (by grind) BareContainer.compare]
-        simp only [List.compareLex.into_attachWithSize.aux l2 l3 (max (max (sizeOf l1) (sizeOf l2)) (sizeOf l3)) (by grind) BareContainer.compare]
-        simp only [List.compareLex.into_attachWithSize.aux l1 l3 (max (max (sizeOf l1) (sizeOf l2)) (sizeOf l3)) (by grind) BareContainer.compare]
-        apply List.compareLex.isLE_trans
-        · intro ⟨a, h_a⟩ ⟨b, h_b⟩
-          dsimp only
-          apply BareContainer.compare.eq_swap
-        intro ⟨a, h_a⟩ ⟨b, h_b⟩ ⟨c, h_c⟩
+  · contradiction
+  split at h23 <;> rename_i h_id23
+  · grind
+  · contradiction
+  have h_id12_eq := Std.LawfulEqOrd.eq_of_compare h_id12
+  have h_id23_eq := Std.LawfulEqOrd.eq_of_compare h_id23
+  subst h_id12_eq
+  subst h_id23_eq
+  dsimp only at *
+  rewrite [h_id12]
+  dsimp only
+  split at h12 <;> rename_i h_data12
+  · split at h23 <;> rename_i h_data23
+    · have h_data12_eq := Std.LawfulEqOrd.eq_of_compare h_data12
+      have h_data23_eq := Std.LawfulEqOrd.eq_of_compare h_data23
+      subst h_data12_eq
+      subst h_data23_eq
+      simp only [h_data12]
+      revert h12 h23
+      simp only [Array.compareLex_eq_compareLex_toList]
+      apply transLeToLt
+      · apply List.compareLex.eq_of_compare
+        · apply BareContainer.compare.compare_self
+        · apply BareContainer.compare.eq_of_compare
+      · apply List.compareLex.eq_swap
+        apply BareContainer.compare.eq_swap
+      simp only [List.compareLex.into_attachWithSize.aux l1 l2 (max (max (sizeOf l1) (sizeOf l2)) (sizeOf l3)) (by grind) BareContainer.compare]
+      simp only [List.compareLex.into_attachWithSize.aux l2 l3 (max (max (sizeOf l1) (sizeOf l2)) (sizeOf l3)) (by grind) BareContainer.compare]
+      simp only [List.compareLex.into_attachWithSize.aux l1 l3 (max (max (sizeOf l1) (sizeOf l2)) (sizeOf l3)) (by grind) BareContainer.compare]
+      apply List.compareLex.isLE_trans
+      · intro ⟨a, h_a⟩ ⟨b, h_b⟩
         dsimp only
-        apply BareContainer.compare.isLE_trans
-      · grind
-    · split at h23 <;> rename_i h_data23
-      · grind
-      · have := Std.TransCmp.lt_trans h12 h23
-        grind
+        apply BareContainer.compare.eq_swap
+      intro ⟨a, h_a⟩ ⟨b, h_b⟩ ⟨c, h_c⟩
+      dsimp only
+      apply BareContainer.compare.isLE_trans
+    · grind
+  · split at h23 <;> rename_i h_data23
+    · grind
+    · have := Std.TransCmp.lt_trans h12 h23
+      grind
 termination_by (max (max (sizeOf x1) (sizeOf x2)) (sizeOf x3))
 decreasing_by
   simp_all
@@ -417,8 +423,8 @@ def Container.compare
   [∀ id, Ord (ctors id).Data]
   (x1 x2: Container ctors)
   : Ordering
-  :=
-    BareContainer.compare x1.val x2.val
+:=
+  BareContainer.compare x1.val x2.val
 
 /-
   Theorems on Container.compare
@@ -431,10 +437,10 @@ theorem Container.compare.compare_self
   [∀ id, Std.ReflOrd (ctors id).Data]
   (x: Container ctors)
   : compare x x = .eq
-  := by
-    cases x
-    simp [Container.compare]
-    apply BareContainer.compare.compare_self
+:= by
+  cases x
+  simp [Container.compare]
+  apply BareContainer.compare.compare_self
 
 theorem Container.compare.eq_of_compare
   {CtorId} {ctors: Ctors CtorId}
@@ -443,11 +449,11 @@ theorem Container.compare.eq_of_compare
   [∀ id, Std.LawfulEqOrd (ctors id).Data]
   (x1 x2: Container ctors)
   : compare x1 x2 = .eq → x1 = x2
-  := by
-    cases x1; cases x2
-    rewrite [Subtype.mk.injEq]
-    simp [Container.compare]
-    apply BareContainer.compare.eq_of_compare
+:= by
+  cases x1; cases x2
+  rewrite [Subtype.mk.injEq]
+  simp [Container.compare]
+  apply BareContainer.compare.eq_of_compare
 
 theorem Container.compare.eq_swap
   {CtorId} {ctors: Ctors CtorId}
@@ -457,10 +463,10 @@ theorem Container.compare.eq_swap
   [∀ id, Std.OrientedOrd (ctors id).Data]
   (x1 x2: Container ctors)
   : compare x1 x2 = (compare x2 x1).swap
-  := by
-    cases x1; cases x2
-    simp [Container.compare]
-    apply BareContainer.compare.eq_swap
+:= by
+  cases x1; cases x2
+  simp [Container.compare]
+  apply BareContainer.compare.eq_swap
 
 theorem Container.compare.isLE_trans
   {CtorId} {ctors: Ctors CtorId}
@@ -471,40 +477,33 @@ theorem Container.compare.isLE_trans
   [∀ id, Std.TransOrd (ctors id).Data]
   (x1 x2 x3: Container ctors)
   : (compare x1 x2).isLE → (compare x2 x3).isLE → (compare x1 x3).isLE
-  := by
-    cases x1; cases x2; cases x3
-    simp [Container.compare]
-    apply BareContainer.compare.isLE_trans
-
+:= by
+  cases x1; cases x2; cases x3
+  simp [Container.compare]
+  apply BareContainer.compare.isLE_trans
 
 class RepresentableOrd (f: Type → Type) [FunctorSizeOf f] [Representable f] where
-  ctoridOrd: Ord (Representable.CtorId f)
-  := by
+  ctoridOrd: Ord (Representable.CtorId f) := by
     simp only [ALaCarte.Representable.CtorId]
     exact inferInstance
-  ctoridOrd_lawfulEq: Std.LawfulEqOrd (Representable.CtorId f)
-  := by
+  ctoridOrd_lawfulEq: Std.LawfulEqOrd (Representable.CtorId f) := by
     simp only [ALaCarte.Representable.CtorId]
     exact inferInstance
-  ctoridOrd_trans: Std.TransOrd (Representable.CtorId f)
-  := by
+  ctoridOrd_trans: Std.TransOrd (Representable.CtorId f) := by
     simp only [ALaCarte.Representable.CtorId]
     exact inferInstance
 
-  ctorDataOrd: ∀ id, Ord (Representable.ctors (f := f) id).Data
-  := by
+  ctorDataOrd: ∀ id, Ord (Representable.ctors (f := f) id).Data := by
     intro id
     simp only [ALaCarte.Representable.ctors]
     cases id <;>
     exact inferInstance
-  ctorDataOrd_lawfulEq: ∀ id, Std.LawfulEqOrd (Representable.ctors (f := f) id).Data
-  := by
+  ctorDataOrd_lawfulEq: ∀ id, Std.LawfulEqOrd (Representable.ctors (f := f) id).Data := by
     intro id
     simp only [ALaCarte.Representable.ctors]
     cases id <;>
     exact inferInstance
-  ctorDataOrd_trans: ∀ id, Std.TransOrd (Representable.ctors (f := f) id).Data
-  := by
+  ctorDataOrd_trans: ∀ id, Std.TransOrd (Representable.ctors (f := f) id).Data := by
     intro id
     simp only [ALaCarte.Representable.ctors]
     cases id <;>
@@ -542,16 +541,16 @@ def FunctorUnion.CtorId.compare
   [∀ id, FunctorSizeOf (fs id)] [∀ id, Representable (fs id)] [∀ id, RepresentableOrd (fs id)]
   (x1 x2: FunctorUnion.CtorId fs)
   : Ordering
-  :=
-    let { idHead := idHead1, idTail := idTail1 } := x1
-    let { idHead := idHead2, idTail := idTail2 } := x2
-    match h: Ord.compare idHead1 idHead2 with
-    | .lt => .lt
-    | .gt => .gt
-    | .eq => by
-      simp at h
-      subst h
-      exact (Ord.compare idTail1 idTail2)
+:=
+  let { idHead := idHead1, idTail := idTail1 } := x1
+  let { idHead := idHead2, idTail := idTail2 } := x2
+  match h: Ord.compare idHead1 idHead2 with
+  | .lt => .lt
+  | .gt => .gt
+  | .eq => by
+    simp at h
+    subst h
+    exact (Ord.compare idTail1 idTail2)
 
 theorem FunctorUnion.CtorId.compare.compare_self
   {a: Type}
@@ -560,12 +559,12 @@ theorem FunctorUnion.CtorId.compare.compare_self
   [∀ id, FunctorSizeOf (fs id)] [∀ id, Representable (fs id)] [∀ id, RepresentableOrd (fs id)]
   (x: FunctorUnion.CtorId fs)
   : compare x x = .eq
-  := by
-    let {idHead, idTail} := x
-    simp only [compare]
-    have idHead_refl: Ord.compare idHead idHead = .eq := by simp
-    rewrite [idHead_refl]
-    simp
+:= by
+  let {idHead, idTail} := x
+  simp only [compare]
+  have idHead_refl: Ord.compare idHead idHead = .eq := by simp
+  rewrite [idHead_refl]
+  simp
 
 theorem FunctorUnion.CtorId.compare.eq_of_compare
   {a: Type}
@@ -574,16 +573,16 @@ theorem FunctorUnion.CtorId.compare.eq_of_compare
   [∀ id, FunctorSizeOf (fs id)] [∀ id, Representable (fs id)] [∀ id, RepresentableOrd (fs id)]
   (x1 x2: FunctorUnion.CtorId fs)
   : compare x1 x2 = .eq → x1 = x2
-  := by
-    let { idHead := idHead1, idTail := idTail1 } := x1
-    let { idHead := idHead2, idTail := idTail2 } := x2
-    simp only [compare]
-    split
-    · grind
-    · grind
-    · have : idHead1 = idHead2 := by grind
-      subst this
-      grind
+:= by
+  let { idHead := idHead1, idTail := idTail1 } := x1
+  let { idHead := idHead2, idTail := idTail2 } := x2
+  simp only [compare]
+  split
+  · grind
+  · grind
+  · have : idHead1 = idHead2 := by grind
+    subst this
+    grind
 
 theorem FunctorUnion.CtorId.compare.eq_swap
   {a: Type}
@@ -592,19 +591,19 @@ theorem FunctorUnion.CtorId.compare.eq_swap
   [∀ id, FunctorSizeOf (fs id)] [∀ id, Representable (fs id)] [∀ id, RepresentableOrd (fs id)]
   (x1 x2: FunctorUnion.CtorId fs)
   : compare x1 x2 = (compare x2 x1).swap
-  := by
-    let { idHead := idHead1, idTail := idTail1 } := x1
-    let { idHead := idHead2, idTail := idTail2 } := x2
-    simp only [compare]
-    have idHead_swap: Ord.compare idHead1 idHead2 = (Ord.compare idHead2 idHead1).swap := Std.OrientedOrd.eq_swap
-    split
-    · split <;> grind
-    · split <;> grind
-    have heq: idHead1 = idHead2 := by grind
-    subst heq
-    dsimp only
-    have idTail_swap: Ord.compare idTail1 idTail2 = (Ord.compare idTail2 idTail1).swap := Std.OrientedOrd.eq_swap
-    split <;> grind
+:= by
+  let { idHead := idHead1, idTail := idTail1 } := x1
+  let { idHead := idHead2, idTail := idTail2 } := x2
+  simp only [compare]
+  have idHead_swap: Ord.compare idHead1 idHead2 = (Ord.compare idHead2 idHead1).swap := Std.OrientedOrd.eq_swap
+  split
+  · split <;> grind
+  · split <;> grind
+  have heq: idHead1 = idHead2 := by grind
+  subst heq
+  dsimp only
+  have idTail_swap: Ord.compare idTail1 idTail2 = (Ord.compare idTail2 idTail1).swap := Std.OrientedOrd.eq_swap
+  split <;> grind
 
 theorem FunctorUnion.CtorId.compare.isLE_trans
   {a: Type}
@@ -613,32 +612,32 @@ theorem FunctorUnion.CtorId.compare.isLE_trans
   [∀ id, FunctorSizeOf (fs id)] [∀ id, Representable (fs id)] [∀ id, RepresentableOrd (fs id)]
   (x1 x2 x3: FunctorUnion.CtorId fs)
   : (compare x1 x2).isLE → (compare x2 x3).isLE → (compare x1 x3).isLE
-  := by
-    let { idHead := idHead1, idTail := idTail1 } := x1
-    let { idHead := idHead2, idTail := idTail2 } := x2
-    let { idHead := idHead3, idTail := idTail3 } := x3
-    apply transLtToLe
-    · apply FunctorUnion.CtorId.compare.eq_of_compare
-    simp only [compare]
-    intro h12 h23
-    split at h12 <;> rename_i h_idHead12
-    · split at h23 <;> rename_i h_idHead23
-      · have := Std.TransCmp.lt_trans h_idHead12 h_idHead23
-        grind
-      · contradiction
-      · grind
+:= by
+  let { idHead := idHead1, idTail := idTail1 } := x1
+  let { idHead := idHead2, idTail := idTail2 } := x2
+  let { idHead := idHead3, idTail := idTail3 } := x3
+  apply transLtToLe
+  · apply FunctorUnion.CtorId.compare.eq_of_compare
+  simp only [compare]
+  intro h12 h23
+  split at h12 <;> rename_i h_idHead12
+  · split at h23 <;> rename_i h_idHead23
+    · have := Std.TransCmp.lt_trans h_idHead12 h_idHead23
+      grind
     · contradiction
-    · split at h23 <;> rename_i h_idHead23
-      · grind
-      · contradiction
-      · have h_idHead12_eq := Std.LawfulEqOrd.eq_of_compare h_idHead12
-        have h_idHead23_eq := Std.LawfulEqOrd.eq_of_compare h_idHead23
-        subst h_idHead12_eq
-        subst h_idHead23_eq
-        dsimp only at *
-        rewrite [h_idHead12]
-        dsimp only
-        exact Std.TransCmp.lt_trans h12 h23
+    · grind
+  · contradiction
+  · split at h23 <;> rename_i h_idHead23
+    · grind
+    · contradiction
+    · have h_idHead12_eq := Std.LawfulEqOrd.eq_of_compare h_idHead12
+      have h_idHead23_eq := Std.LawfulEqOrd.eq_of_compare h_idHead23
+      subst h_idHead12_eq
+      subst h_idHead23_eq
+      dsimp only at *
+      rewrite [h_idHead12]
+      dsimp only
+      exact Std.TransCmp.lt_trans h12 h23
 
 instance {a: Type} [Ord a] [Std.LawfulEqOrd a] [Std.TransOrd a] (fs: a → Type → Type) [∀ id, FunctorSizeOf (fs id)] [∀ id, Representable (fs id)] [∀ id, RepresentableOrd (fs id)]: RepresentableOrd (FunctorUnion fs) where
   ctoridOrd := {
