DY/Bytes/AttackerKnowledgeTheorem.lean
@@ -30,12 +30,12 @@ instance
   (atts: t → SubAttackerKnowledge SubF)
   [pfs: ∀ id, SubAttackerKnowledgeTheorem (atts id)]
   : SubAttackerKnowledgeTheorem (SubAttackerKnowledge.combine' atts)
-  where
-    pf := by
-      intro b tr h_tr
-      apply SubAttackerKnowledge.combine'.implies
-      intro id b
-      exact (pfs id).pf b tr h_tr
+where
+  pf := by
+    intro b tr h_tr
+    apply SubAttackerKnowledge.combine'.implies
+    intro id b
+    exact (pfs id).pf b tr h_tr
 
 instance
   {t: Type}
@@ -43,12 +43,12 @@ instance
   (atts: ∀ id, SubAttackerKnowledge (SubFs id))
   [pfs: ∀ id, SubAttackerKnowledgeTheorem (atts id)]
   : SubAttackerKnowledgeTheorem (SubAttackerKnowledge.combine atts)
-  where
-    pf := by
-      intro b tr h_tr
-      apply SubAttackerKnowledge.combine.implies
-      intro id b
-      exact (pfs id).pf b tr h_tr
+where
+  pf := by
+    intro b tr h_tr
+    apply SubAttackerKnowledge.combine.implies
+    intro id b
+    exact (pfs id).pf b tr h_tr
 
 end AttackerKnowledgeTheorem
 
@@ -58,16 +58,15 @@ theorem Bytes.AttackerKnows_implies_Publishable
   [AttackerKnowledge]
   [inst: AttackerKnowledgeTheorem]
   (b: Bytes) (tr: ProofTrace)
-  :
-    tr.invariant →
+  : tr.invariant →
     Bytes.AttackerKnows b tr →
     b.Publishable tr
-  := by
-    intro h_tr
-    apply Bytes.AttackerKnows.is_least_fixpoint (·.Publishable tr) b tr
-    · intro b
-      exact inst.inst.pf b tr h_tr
-    · intro b
-      exact Bytes.MessageSent_implies_Publishable b tr h_tr
+:= by
+  intro h_tr
+  apply Bytes.AttackerKnows.is_least_fixpoint (·.Publishable tr) b tr
+  · intro b
+    exact inst.inst.pf b tr h_tr
+  · intro b
+    exact Bytes.MessageSent_implies_Publishable b tr h_tr
 
 end DY
