DY/EquationalTheory/Concat.lean
@@ -76,16 +76,16 @@ instance: CanConcat Bytes where
 theorem split_concat
   (lhs rhs: Bytes)
   : split (concat lhs rhs) (lhs.length) = some (lhs, rhs)
-  := by
-    simp only [split, concat]
-    grind
+:= by
+  simp only [split, concat]
+  grind
 
 theorem concat_split
   (buf: Bytes) (i: Nat) (lhs rhs: Bytes)
   : split buf i = some (lhs, rhs) → concat lhs rhs = buf
-  := by
-    simp only [concat, split]
-    grind
+:= by
+  simp only [concat, split]
+  grind
 
 end Constructors
 
@@ -129,37 +129,35 @@ variable [AttackerKnowledge] [AttackerKnowledge.Has attackerKnowledge]
 
 theorem attacker_knows_concat
   (lhs rhs: Bytes) (tr: Trace α)
-  :
-    lhs.AttackerKnows tr →
+  : lhs.AttackerKnows tr →
     rhs.AttackerKnows tr →
     (concat lhs rhs).AttackerKnows tr
-  := by
-    intro h_lhs h_rhs
-    apply Bytes.AttackerKnows.prove attKnowsConcat
-    simp only [attKnowsConcat, Kleene.Forall]
-    grind
+:= by
+  intro h_lhs h_rhs
+  apply Bytes.AttackerKnows.prove attKnowsConcat
+  simp only [attKnowsConcat, Kleene.Forall]
+  grind
 
 theorem attacker_knows_split
   (buf: Bytes) (i: Nat) (tr: Trace α)
-  :
-    buf.AttackerKnows tr →
+  : buf.AttackerKnows tr →
     match split buf i with
     | none => True
     | some (lhs, rhs) =>
       lhs.AttackerKnows tr ∧
       rhs.AttackerKnows tr
-  := by
-    intro h_buf
-    split
-    · trivial
-    rename_i lhs rhs _
-    constructor
-    · apply Bytes.AttackerKnows.prove attKnowsSplitLeft
-      simp only [attKnowsSplitLeft, Kleene.Forall]
-      grind
-    · apply Bytes.AttackerKnows.prove attKnowsSplitRight
-      simp only [attKnowsSplitRight, Kleene.Forall]
-      grind
+:= by
+  intro h_buf
+  split
+  · trivial
+  rename_i lhs rhs _
+  constructor
+  · apply Bytes.AttackerKnows.prove attKnowsSplitLeft
+    simp only [attKnowsSplitLeft, Kleene.Forall]
+    grind
+  · apply Bytes.AttackerKnows.prove attKnowsSplitRight
+    simp only [attKnowsSplitRight, Kleene.Forall]
+    grind
 
 end AttackerKnowledge
 
@@ -191,72 +189,67 @@ variable [BytesLength]
 @[simp]
 theorem concat.WellFormed
   (lhs rhs: Bytes) (tr: ProofTrace)
-  :
-    (concat lhs rhs).WellFormed tr = (lhs.WellFormed tr ∧ rhs.WellFormed tr)
-  := by
-    simp [concat, Bytes.WellFormed.eq, Concat.invariants]
+  : (concat lhs rhs).WellFormed tr = (lhs.WellFormed tr ∧ rhs.WellFormed tr)
+:= by
+  simp [concat, Bytes.WellFormed.eq, Concat.invariants]
 
 @[simp]
 theorem concat.label
   (lhs rhs: Bytes) (tr: ProofTrace)
   : (concat lhs rhs).label tr = Label.meet (lhs.label tr) (rhs.label tr)
-  := by
-    simp [concat, Bytes.label.eq, Concat.invariants]
+:= by
+  simp [concat, Bytes.label.eq, Concat.invariants]
 
 @[simp]
 theorem concat.Invariant
   (lhs rhs: Bytes) (tr: ProofTrace)
   : (concat lhs rhs).Invariant tr = (lhs.Invariant tr ∧ rhs.Invariant tr)
-  := by
-    simp [concat, Bytes.Invariant.eq, Concat.invariants]
-
+:= by
+  simp [concat, Bytes.Invariant.eq, Concat.invariants]
 
 @[simp]
 theorem split.WellFormed
   (buf: Bytes) (i: Nat) (tr: ProofTrace)
-  :
-    match split buf i with
+  : match split buf i with
     | none => True
     | some (lhs, rhs) =>
       buf.WellFormed tr = (lhs.WellFormed tr ∧ rhs.WellFormed tr)
-  := by
-    split
-    · trivial
-    rename_i lhs rhs heq
-    rewrite [← concat_split buf i lhs rhs heq]
-    simp
+:= by
+  split
+  · trivial
+  rename_i lhs rhs heq
+  rewrite [← concat_split buf i lhs rhs heq]
+  simp
 
 @[simp]
 theorem split.label
   (buf: Bytes) (i: Nat) (tr: ProofTrace)
-  :
-    match split buf i with
+  : match split buf i with
     | none => True
     | some (lhs, rhs) =>
       buf.label tr = Label.meet (lhs.label tr) (rhs.label tr)
-  := by
-    split
-    · trivial
-    rename_i lhs rhs heq
-    rewrite [← concat_split buf i lhs rhs heq]
-    simp
+:= by
+  split
+  · trivial
+  rename_i lhs rhs heq
+  rewrite [← concat_split buf i lhs rhs heq]
+  simp
 
 @[simp]
 theorem split.Invariant
   (buf: Bytes) (i: Nat) (tr: ProofTrace)
-  :
-    buf.Invariant tr →
+  : buf.Invariant tr →
     match split buf i with
     | none => True
     | some (lhs, rhs) =>
       lhs.Invariant tr ∧ rhs.Invariant tr
-  := by
-    intro h_buf
-    split
-    · trivial
-    rename_i lhs rhs heq
-    rewrite [← concat_split buf i lhs rhs heq] at h_buf
-    simp_all
+:= by
+  intro h_buf
+  split
+  · trivial
+  rename_i lhs rhs heq
+  rewrite [← concat_split buf i lhs rhs heq] at h_buf
+  simp_all
 
 end Invariants
 
